ML_SP_Soundness.v
@@ -93,27 +93,23 @@ Qed.
 
 Lemma well_subst_fresh : forall K K' K'' S Ys L1 M,
   well_subst (K & K' & K'') (K & map (kind_subst S) K'') S ->
-  fresh (L1 \u dom S \u dom (K & K'')) (length (sch_kinds M)) Ys ->
-  well_subst (K & K' & K'' & kinds_open_vars (sch_kinds M) Ys)
+  fresh (L1 \u dom S \u dom (K & K' & K'')) (length (sch_kinds M)) Ys ->
+  well_subst (K & K' & (K'' & kinds_open_vars (sch_kinds M) Ys))
     (K & map (kind_subst S) (K'' & kinds_open_vars (sch_kinds M) Ys)) S.
 Proof.
   introv WS Fr.
-  assert (KxYs: disjoint (dom K \u dom K'')
-                         (dom (kinds_open_vars (sch_kinds M) Ys))).
-    unfold kinds_open_vars.
-    intro v.
-    destruct* (in_vars_dec v (dom K \u dom K'')).
-    right; intro.
-    elim (fresh_rev _ _ Fr (x:=v)).
-    rewrite* dom_concat. auto with sets.
-    apply (in_dom_combine _ _ H0).
   intro x; intros.
-  rewrite map_concat. rewrite <- concat_assoc.
+  rewrite map_concat. rewrite <- concat_assoc in *.
   destruct* (binds_concat_inv H) as [[N B]|B]; clear H.
     apply* well_kinded_extend.
     rewrite dom_map. rewrite dom_concat; rewrite* dom_map.
-  destruct k; try constructor.
-  simpl. rewrite get_notin_dom.
+    unfold kinds_open_vars. rewrite mkset_dom.
+    apply disjoint_comm. apply* (fresh_disjoint (length (sch_kinds M))).
+    rewrite dom_concat in Fr. rewrite dom_concat in Fr. auto*.
+    unfold kinds_open. rewrite map_length.
+    rewrite* <- (fresh_length _ _ _ Fr).
+  destruct k; simpl; try apply* wk_any.
+  rewrite get_notin_dom.
     apply* wk_kind. apply* binds_prepend.
       use (binds_map (kind_subst S) B).
       simpl in H; apply H.
@@ -145,18 +141,196 @@ Proof.
   elim (binds_fresh B0). apply get_none_notin. apply* map_get_none.
 Qed.
 
-Lemma typing_typ_subst : forall F K'' S K K' E t T,
+Definition env_equiv (A : Set) (E F : Env.env A) :=
+  ok F /\ forall x a, binds x a E <-> binds x a F.
+
+Lemma env_equiv_rev : forall (A : Set) (E F : Env.env A),
+  env_equiv E F -> ok E -> env_equiv F E.
+Proof.
+  intros; split*.
+  destruct H.
+  intros. destruct* (H1 x a).
+Qed.
+
+Lemma env_equiv_dom : forall (A : Set) (E F : Env.env A),
+  env_equiv E F -> dom E << dom F.
+Proof.
+  intros. intros x Hx.
+  destruct H.
+  case_eq (get x E); intros.
+    use (proj1 (H0 x a) H1).
+    case_eq (S.mem x (dom F)); intros. apply* S.mem_2.
+    elim (binds_fresh H2). intro. rewrite (S.mem_1 H4) in H3. discriminate.
+  elim (get_none_notin _ H1 Hx).
+Qed.
+  
+Lemma kenv_ok_equiv : forall K K',
+  kenv_ok K -> env_equiv K K' -> kenv_ok K'.
+Proof.
+  intros K K' [Ok Kok] [Ok' EQ].
+  split*.
+  intros x a B.
+  apply (Kok x a).
+  apply* (proj2 (EQ x a)).
+Qed.
+
+Lemma For_all2_imp : forall (A B:Set) (P P':A->B->Prop) l1 l2,
+  (forall x y, P x y -> P' x y) ->
+  For_all2 P l1 l2 ->
+  For_all2 P' l1 l2.
+Proof.
+  induction l1; introv; elim l2; simpls; auto*.
+Qed.
+
+Lemma proper_instance_equiv : forall K K' M Us,
+  proper_instance K M Us -> env_equiv K K' -> proper_instance K' M Us.
+Proof.
+  introv; intros [Hty [Hsc WK]] [Ok' EQ].
+  split*.
+  split*.
+  apply* (For_all2_imp (well_kinded K)).
+  intros.
+  inversions H. constructor.
+  apply* wk_kind.
+  apply* (proj1 (EQ x0 (Some k'))).
+Qed.
+
+Lemma well_subst_equiv : forall K K' K0 S,
+  well_subst K K0 S -> env_equiv K K' -> well_subst K' K0 S.
+Proof.
+  introv; intros WS [_ EQ].
+  intro; intros.
+  apply* (WS Z).
+  apply* (proj2 (EQ Z k)).
+Qed.
+
+Fixpoint env_remove (A:Set) (E : Env.env A) (V : vars) {struct E} : Env.env A :=
+  match E with
+  | nil => nil
+  | (x,a) :: E' =>
+      if S.mem x V then env_remove E' V else (x,a) :: env_remove E' V
+  end.
+
+Lemma dom_remove : forall (A:Set) V (F:Env.env A),
+  dom (env_remove F V) << dom F /\
+  disjoint (dom (env_remove F V)) V /\
+  dom F << dom (env_remove F V) \u V.
+Proof.
+  induction F. simpl. split3; intro; auto.
+    intro H. elim (in_empty H).
+  destruct a.
+  simpl.
+  destruct IHF as [IH1 [IH2 IH3]].
+  case_eq (S.mem v V); intros.
+    split3*; intros x Hx.
+    apply* S.union_3.
+    destruct* (S.union_1 Hx).
+    apply* S.union_3.
+    rewrite (proj1 (in_singleton _ _) H0).
+    apply* S.mem_2.
+  simpl; split3.
+    intros x Hx.
+    destruct* (S.union_1 Hx).
+      apply* S.union_2.
+      apply* S.union_3.
+    apply* disjoint_union.
+      intro.
+      destruct (x == v).
+        rewrite e; right; intro. rewrite (S.mem_1 H0) in H. discriminate.
+      left. intro; elim n. apply (proj1 (in_singleton _ _) H0).
+    intros x Hx.
+    rewrite <- union_assoc.
+    destruct* (S.union_1 Hx).
+      apply* S.union_2.
+      apply* S.union_3.
+Qed.
+
+Lemma env_remove_ok : forall (A:Set) (E F:Env.env A),
+  ok E -> ok F -> ok (E & env_remove F (dom E)).
+Proof.
+  induction F; simpl; intros. auto.
+  destruct a.
+  case_eq (S.mem v (dom E)); intros.
+    inversions H0. auto.
+  replace ((v,a) :: env_remove F (dom E))
+    with (env_remove F (dom E) & iter_push (v :: nil) (a :: nil))
+    by (simpl; auto).
+  rewrite <- concat_assoc.
+  inversions H0.
+  apply* ok_concat_iter_push.
+  rewrite dom_concat.
+  apply* fresh_union_l.
+    simpl. split*.
+    intro. rewrite (S.mem_1 H2) in H1. discriminate.
+  destruct (dom_remove (dom E) F) as [HR1 [HR2 HR3]].
+  apply* fresh_sub.
+Qed.
+
+Lemma env_remove_binds : forall (A:Set) V x y (E:Env.env A),
+  binds x y (env_remove E V) -> binds x y E.
+Proof.
+  induction E; simpl; intros. auto.
+  destruct a; unfold binds; simpl.
+  destruct (dom_remove V E) as [HR1 [HR2 HR3]].
+  case_eq (S.mem v V); intros; rewrite H0 in H.
+    destruct* (x == v). 
+    destruct (HR2 x).
+    elim (binds_fresh H H1).
+    rewrite <- e in H0. elim (H1 (S.mem_2 H0)).
+  unfold binds in H; simpl in H.
+  destruct* (x == v).
+Qed.
+
+Lemma binds_in_dom : forall A x a (E:Env.env A),
+  binds x a E -> x \in dom E.
+Proof.
+  induction E; unfold binds; simpl; intros.
+    discriminate.
+  destruct a0. destruct (x == v).
+    apply S.union_2. apply* (proj2 (in_singleton x v)).
+  apply* S.union_3.
+Qed.
+
+Lemma env_remove_equiv : forall (A:Set) (E F:Env.env A),
+  ok E -> ok F -> extends E F -> env_equiv F (E & env_remove F (dom E)).
+Proof.
+  intros.
+  split.
+    apply* env_remove_ok.
+  intros; split; intro.
+  destruct (dom_remove (dom E) F) as [HR1 [HR2 HR3]].
+  case_eq (get x (E & env_remove F (dom E))); intros.
+    binds_cases H3.
+      apply* binds_concat_ok.
+      use (H1 x a0 B).
+      rewrite (binds_func H3 H2) in B. auto.
+      apply* env_remove_ok.
+    use (env_remove_binds _ _ B0).
+    rewrite (binds_func H3 H2) in B0. auto.
+  elim (get_none_notin _ H3).
+  rewrite dom_concat.
+  rewrite union_comm.
+  apply (HR3 x).
+  apply* binds_in_dom.
+  binds_cases H2.
+    apply* H1.
+  apply* env_remove_binds.
+Qed.
+
+Lemma typing_typ_subst : forall F K1 K'' S K K' E t T,
+  env_equiv K1 (K & K' & K'') ->
   disjoint (dom S) (env_fv E \u fv_in kind_fv K) ->
   env_prop type S ->
-  well_subst (K & K' & K'') (K & map (kind_subst S) K'') S ->
-  K & K' & K''; E & F |= t ~: T -> 
+  well_subst K1 (K & map (kind_subst S) K'') S ->
+  K1; E & F |= t ~: T -> 
   K & map (kind_subst S) K''; E & (map (sch_subst S) F) |= t ~: (typ_subst S T).
 Proof.
-  introv. intros Dis TS WS Typ.
-  gen_eq (K & K' & K'') as GK; gen_eq (E & F) as G; gen K''; gen F.
-  induction Typ; introv WS EQ EQ'; subst; simpls typ_subst.
+  introv GK Dis TS WS Typ.
+  gen_eq (E & F) as G; gen K''; gen F.
+  induction Typ; introv EQ WS EQ'; subst; simpls typ_subst.
+  (* Var *)
   rewrite~ sch_subst_open. apply* typing_var.
-    apply* kenv_ok_subst.
+    apply* kenv_ok_subst. apply* kenv_ok_equiv.
     binds_cases H1.
       apply* binds_concat_fresh.
        rewrite* sch_subst_fresh. use (fv_in_spec sch_fv B).
@@ -164,29 +338,81 @@ Proof.
        destruct* (proj1 (notin_union _ _ _) H3).
       auto*.
     apply* proper_instance_subst.
+    apply* proper_instance_equiv.
+    apply* well_subst_equiv.
+  (* Abs *)
   apply_fresh* typing_abs as y.
    assert (r: Sch (typ_subst S U) nil = sch_subst S (Sch U nil)); auto.
    rewrite r; apply_ih_map_bind* H1.
-  apply_fresh* (@typing_let (sch_subst S M) (L1 \u dom S \u dom (K&K''))) as y.
+  (* Let *)
+  apply_fresh* (@typing_let (sch_subst S M) (L1 \u dom S \u dom (K&K'&K'')))
+      as y.
+   assert (Kok: kenv_ok K0).
+     pick_fresh y. assert (y \notin L2) by auto.
+     use (H1 y H3).
    clear H H1 H2. clear L2 T2 t2 Dis.
    simpl. intros Ys Fr. 
    rewrite* <- sch_subst_open_vars.
    rewrite* <- kinds_subst_open_vars.
    rewrite concat_assoc. rewrite <- map_concat.
    unfold sch_arity in Fr; simpl in Fr; rewrite map_length in Fr.
+    assert (EQ': env_equiv (K0 & kinds_open_vars (sch_kinds M) Ys)
+                (K & K' & (K'' & kinds_open_vars (sch_kinds M) Ys))).
+     clear H0 WS TS t1 E F.
+     destruct EQ; split.
+     unfold concat. rewrite app_ass.
+     change (ok (K & K' & K'' & kinds_open_vars (sch_kinds M) Ys)).
+     apply* disjoint_ok. unfold kinds_open_vars. apply* ok_combine_fresh.
+     unfold kinds_open_vars. rewrite mkset_dom.
+     apply disjoint_comm. apply* (fresh_disjoint (length (sch_kinds M))).
+     unfold kinds_open. rewrite map_length.
+     rewrite* <- (fresh_length _ _ _ Fr).
+     intros. destruct (H0 x a); clear H0.
+     split; intro B; binds_cases B; auto*.
+     apply* binds_concat_fresh. destruct* (proj1 (notin_union _ _ _) Fr0).
+     apply* binds_concat_fresh. destruct* (proj1 (notin_union _ _ _) Fr0).
    apply* H0; clear H0.
+     assert (ok (K0 & kinds_open_vars (sch_kinds M) Ys)).
+       apply* disjoint_ok. unfold kinds_open_vars. apply* ok_combine_fresh.
+       unfold kinds_open_vars. rewrite mkset_dom.
+       apply disjoint_comm. apply* (fresh_disjoint (length (sch_kinds M))).
+       use (env_equiv_dom EQ).
+       apply* fresh_sub.
+       apply* subset_trans.
+       apply subset_union_weak_r.
+       unfold kinds_open. rewrite map_length.
+       rewrite* <- (fresh_length _ _ _ Fr).
+     use (env_equiv_rev EQ' H).
+     apply* well_subst_equiv.
      apply* well_subst_fresh.
-   rewrite* concat_assoc.
-  apply_ih_map_bind* H2.
+     apply* well_subst_equiv.
+   apply_ih_map_bind* H2.
+  (* App *)
   auto*.
+  (* Cst *)
   rewrite* sch_subst_open.
   assert (disjoint (dom S) (sch_fv (Delta.type c))).
     intro x. rewrite* const_closed.
   rewrite* sch_subst_fresh.
   apply* typing_cst.
     apply* kenv_ok_subst.
+    apply* kenv_ok_equiv.
   rewrite* <- (sch_subst_fresh S H2).
   apply* proper_instance_subst.
+  apply* proper_instance_equiv.
+  apply* well_subst_equiv.
+  (* GC *)
+  assert (exists K2, env_equiv K0 (K & K' & K2)).
+    exists (env_remove K0 (dom(K&K'))).
+    apply* env_remove_equiv.
+    destruct* (ok_concat_inv _ _ (proj1 EQ)).
+    intros x k Hx.
+    apply H0. apply (proj2 (proj2 EQ x k)).
+    apply* binds_concat_ok.
+    apply (proj1 EQ).
+  destruct H2 as [K2 eq2].
+  eapply typing_gc.
+    apply* (IHTyp F K2); clear IHTyp.
 Qed.
 
 Lemma typing_typ_substs : forall K' S K E t T,
